Clean-up of composition and backlifting theories + libraries

src/theory/tools/comp/bir_tsSyntax.sig
@@ -1,0 +1,13 @@
+signature bir_tsSyntax =
+sig
+    include Abbrev
+
+    (************)
+    (* bir_cont *)
+    (*************)
+    val bir_cont_tm    : term
+    val mk_bir_cont    : (term * term * term * term * term * term * term) -> term
+    val dest_bir_cont  : term -> (term * term * term * term * term * term * term)
+    val is_bir_cont    : term -> bool
+
+end
